commit

Src/Prover/Choice.lean
@@ -3,5 +3,33 @@ import Src.Prover.Logic
 namespace prover
 noncomputable section
 
-axiom some {α : Type} {P : α → Prop} : (∃ (x : α), P x) → α
-axiom some_spec {α : Type} {P : α → Prop} (h : ∃ (x : α), P x) : P (some h)
+axiom some {α : Type} [Inhabited α] (P : α → Prop) : α
+axiom some_spec {α : Type} [Inhabited α] {P : α → Prop} (h : ∃ (x : α), P x) : P (some P)
+
+def some' {α : Type} [Inhabited α] {P : α → Prop} (h : ∃ (x : α), P x) : α :=
+some P
+
+section Conditional
+
+theorem exi_ite_val {α : Type} (P : Prop) (x y : α) :
+  ∃ (z : α), (P → z = x) ∧ (¬P → z = y) :=
+prop_rec (λ m => ∃ (z : α), (m → z = x) ∧ (¬m → z = y))
+(exi_intro x # and_intro (λ _ => rfl) (λ h => exfalso # h trivial))
+(exi_intro y # and_intro exfalso (λ _ => rfl))
+
+def ite {α : Type} [Inhabited α] (P : Prop) (x y : α) : α :=
+some' # exi_ite_val P x y
+
+theorem if_pos {α : Type} [Inhabited α] {P : Prop} {x y : α} (h : P) : ite P x y = x :=
+and_left (!some_spec # exi_ite_val P x y) h
+
+theorem if_neg {α : Type} [Inhabited α] {P : Prop} {x y : α} (h : ¬P) : ite P x y = y :=
+and_right (!some_spec # exi_ite_val P x y) h
+
+theorem split_ifs {α : Type} [Inhabited α] (F : α → Prop) {P : Prop} {x y : α}
+  (h₁ : P → F x) (h₂ : ¬P → F y) : F (ite P x y) :=
+or_elim (@em P)
+(λ h₃ => eq_rec' F (if_pos h₃) # h₁ h₃)
+(λ h₃ => eq_rec' F (if_neg h₃) # h₂ h₃)
+
+end Conditional
